LeanMiniscript.lean
@@ -1,5 +1,6 @@
 import LeanMiniscript.Bitcoin.Transaction
 import LeanMiniscript.Bitcoin.TaprootSighash
+import LeanMiniscript.Bitcoin.Schnorr
 import LeanMiniscript.Script.Syntax
 import LeanMiniscript.Script.Assembly
 import LeanMiniscript.Script.ControlFlow
